\documentclass[12pt]{article}
\usepackage{amsmath}
\usepackage{ amssymb }
\usepackage{breqn}
\begin{document}



\section{Linearised Equations}

We begin with the linearised equations from Chris's thesis/papers.


continuity:

\[\frac{\partial  h_1}{\partial  t} + h_0\frac{\partial  u_1}{\partial  x} + u_0\frac{\partial  h_1}{\partial  x} = 0 \]

velocity:

\[\frac{\partial  u_1}{\partial  t} + g\frac{\partial  h_1}{\partial  x} + u_0\frac{\partial  u_1}{\partial  x} - \frac{h_0^2}{3}\left(u_0\frac{\partial^3  u_1}{\partial  x^3} + \frac{\partial^3  u_1}{\partial  x^3 \partial  t}  \right)  = 0 \]

Also G

\[G = u_0h_0 + u_0h_1 + h_0u_1 -\frac{h_0^3}{3} \frac{\partial^2 u_1}{\partial x^2}\]

Now for simplicity, and because its all we need, we assume the water is still (except for the pertubations) so that $u_0 = 0$ thus we get:

\[\frac{\partial  h_1}{\partial  t} + h_0\frac{\partial  u_1}{\partial  x} = 0 \]

\[\frac{\partial  u_1}{\partial  t} + g\frac{\partial  h_1}{\partial  x}  - \frac{h_0^2}{3} \frac{\partial^3  u_1}{\partial  x^3 \partial  t}   = 0 \]

\[G = h_0u_1 -\frac{h_0^3}{3} \frac{\partial^2 u_1}{\partial x^2}\]

Importantly by multiplying the velocity by $h_0$ to get the momentum equation we have

\[\frac{\partial  u_1}{\partial  t}h_0 + g\frac{\partial  h_1}{\partial  x}h_0  - \frac{h_0^3}{3} \frac{\partial^3  u_1}{\partial  x^3 \partial  t}   = 0 \]

and thus

\[\frac{\partial  G}{\partial  t} + g\frac{\partial  h_1}{\partial  x}h_0   = 0 \]

So we finally have 

\[\frac{\partial  h_1}{\partial  t} + h_0\frac{\partial  u_1}{\partial  x} = 0 \]

\[\frac{\partial  G}{\partial  t} + g\frac{\partial  h_1}{\partial  x}h_0   = 0 \]

\[G = h_0u_1 -\frac{h_0^3}{3} \frac{\partial^2 u_1}{\partial x^2}\]

For convenience I will make the following notational changes $H = h_0$, $h = h_1$ and $u = u_1$ . So that 

\[\frac{\partial  h}{\partial  t} + H\frac{\partial  u}{\partial  x} = 0 \]

\[\frac{\partial  G}{\partial  t} + gH\frac{\partial  h}{\partial  x}   = 0 \]

\[G = Hu -\frac{H^3}{3} \frac{\partial^2 u}{\partial x^2}\]

We know that the dispersion relation is given by

\[\omega =  \pm k\sqrt{gH}\sqrt{\frac{3}{k^2H^2 + 3}}\]

\section{Source Term in Mass Equation}

We want to solve this for $u(x_0,t)$ for a given $h(x_0,t)$

\[h_t + Hu_x = 0 \]

\[u_tH + gHh_x - \frac{H^3}{3} u_{xxt}   = 0 \]

\[G = Hu -\frac{H^3}{3} \frac{\partial^2 u}{\partial x^2}\]


The $h(x_0,t)$ is

\begin{multline}
h(x,t)= a_0 \cos\left(2 \pi \left(\frac{x}{\lambda} - \frac{t}{T_0}\right)\right) + \frac{\pi a_0^2}{\lambda} \cos\left(4 \pi \left(\frac{x}{\lambda} - \frac{t}{T_0}\right)\right) \\ - \frac{a_0^3 \pi^2}{2 \lambda^2} \left[\cos\left(2 \pi \left(\frac{x}{\lambda} - \frac{t}{T_0}\right)\right) - \cos\left(6 \pi \left(\frac{x}{\lambda} - \frac{t}{T_0}\right)\right)\right]
\end{multline}

So 
\begin{multline}
h_t(x,t)= \frac{2\pi a_0}{T_0} \sin\left(2 \pi \left(\frac{x}{\lambda} - \frac{t}{T_0}\right)\right) + \frac{4\pi^2 a_0^2}{\lambda T_0} \sin\left(4 \pi \left(\frac{x}{\lambda} - \frac{t}{T_0}\right)\right) \\ - \frac{2a_0^3 \pi^3}{2 \lambda^2 T_0} \left[\sin\left(2 \pi \left(\frac{x}{\lambda} - \frac{t}{T_0}\right)\right) - 3\sin\left(6 \pi \left(\frac{x}{\lambda} - \frac{t}{T_0}\right)\right)\right]
\end{multline}

So we have

\begin{multline}
u_x = -\frac{1}{H}\left[\frac{2\pi a_0}{T_0} \sin\left(2 \pi \left(\frac{x}{\lambda} - \frac{t}{T_0}\right)\right) + \frac{4\pi^2 a_0^2}{\lambda T_0} \sin\left(4 \pi \left(\frac{x}{\lambda} - \frac{t}{T_0}\right)\right) \right] \\ +\frac{1}{H}\left[ \frac{2a_0^3 \pi^3}{2 \lambda^2 T_0} \left[\sin\left(2 \pi \left(\frac{x}{\lambda} - \frac{t}{T_0}\right)\right) - 3\sin\left(6 \pi \left(\frac{x}{\lambda} - \frac{t}{T_0}\right)\right)\right]\right]
\end{multline}


\begin{multline}
u_x = -\frac{1}{H}\left[\frac{2\pi a_0}{T_0} \sin\left(2 \pi \left(\frac{x}{\lambda} - \frac{t}{T_0}\right)\right) + 2\frac{4\pi^2 a_0^2}{\lambda T_0} \sin\left(2 \pi \left(\frac{x}{\lambda} - \frac{t}{T_0}\right)\right) \cos\left(2 \pi \left(\frac{x}{\lambda} - \frac{t}{T_0}\right)\right) \right] \\ +\frac{1}{H}\left[ \frac{2a_0^3 \pi^3}{2 \lambda^2 T_0} \left[\sin\left(2 \pi \left(\frac{x}{\lambda} - \frac{t}{T_0}\right)\right)  -3 \left(-4\sin^3\left(2 \pi \left(\frac{x}{\lambda} - \frac{t}{T_0}\right)\right) + 3\sin\left(2 \pi \left(\frac{x}{\lambda} - \frac{t}{T_0}\right)\right) \right)\right]\right]
\end{multline}

\begin{multline}
u_x = -\frac{\sin\left(2 \pi \left(\frac{x}{\lambda} - \frac{t}{T_0}\right)\right)}{H}\left[\frac{2\pi a_0}{T_0}  + 2\frac{4\pi^2 a_0^2}{\lambda T_0} \cos\left(2 \pi \left(\frac{x}{\lambda} - \frac{t}{T_0}\right)\right) \right] \\ +\frac{\sin\left(2 \pi \left(\frac{x}{\lambda} - \frac{t}{T_0}\right)\right)}{H} \left[ \left[1 -3 \left(-4\sin^2\left(2 \pi \left(\frac{x}{\lambda} - \frac{t}{T_0}\right)\right) + 3 \right)\right]\right]
\end{multline}

\begin{multline}
u_x = -\frac{\sin\left(2 \pi \left(\frac{x}{\lambda} - \frac{t}{T_0}\right)\right)}{H}\left[\frac{2\pi a_0}{T_0}  + 2\frac{4\pi^2 a_0^2}{\lambda T_0} \cos\left(2 \pi \left(\frac{x}{\lambda} - \frac{t}{T_0}\right)\right) \right] \\ +\frac{\sin\left(2 \pi \left(\frac{x}{\lambda} - \frac{t}{T_0}\right)\right)}{H} \left[ \left[ 12\sin^2\left(2 \pi \left(\frac{x}{\lambda} - \frac{t}{T_0}\right)\right) - 8 \right]\right]
\end{multline}

\[
u_x = -\frac{2\sin\left(2 \pi \left(\frac{x}{\lambda} - \frac{t}{T_0}\right)\right)}{H}\left[\frac{\pi a_0}{T_0} -4 + \frac{4\pi^2 a_0^2}{\lambda T_0} \cos\left(2 \pi \left(\frac{x}{\lambda} - \frac{t}{T_0}\right)\right) + 6\sin^2\left(2 \pi \left(\frac{x}{\lambda} - \frac{t}{T_0}\right)\right) \right]
\]













\end{document}
