\documentclass[12pt]{article}
\usepackage{amsmath}
\usepackage{ amssymb }
\usepackage{breqn}
\begin{document}

\title{G for soliton}
\author{Jordan Pitt / u5013521}

\section{Mathematica}

$ (c^2  (\sigma (g + \epsilon^2  \lambda u^2  b_{xx}) h_x + u^{t}(\epsilon + \epsilon \sigma b_x h_x) + \epsilon^2 u (1 + \sigma b_x h_x) u_x +
\sigma h (\epsilon \lambda b_x^2 (u_t + \epsilon u u_x))
+ b_x (g \lambda + \epsilon(\epsilon \lambda^2 u^2 b_{xx} + 0.5\epsilon u_x^2
+ 0.5 u_{xt} + 0.5 \epsilon u u_{xx} ))
+ \epsilon (( 0.5 \epsilon \lambda^2 u^2 b_{xxx} + 0.5 \lambda b_{xx} u_t
+ \sigma h_{x} ( \epsilon u_{x}^2 - u{x,t}) + \epsilon u (1.5 \lambda b_{xx} u_{x} - s h_x u_{xx} )))
+ \epsilon \sigma^2 h^2 ( \frac{1}{3} \epsilon u_{x}u_{xx}
+ \lambda b_x ( 0.5 \epsilon u_x^2 - 0.5 u_{xt} - 0.5 \epsilon u u_{xx})
- \frac{1}{3} u_{xxt} - \frac{1}{3} \epsilon u u_{xxx}))) / l = 0
$ 

$ c^2/l  (\sigma (g + \epsilon^2  \lambda u^2  b_{xx}) h + u^{t}(\epsilon + \epsilon \sigma b_x h_x) + \epsilon^2 u (1 + \sigma b_x h_x) u_x +
\sigma h (\epsilon \lambda b_x^2 (u_t + \epsilon u u_x))
+ b_x (g \lambda + \epsilon(\epsilon \lambda^2 u^2 b_{xx} + 0.5\epsilon u_x^2
+ 0.5 u_{xt} + 0.5 \epsilon u u_{xx} ))
+ \epsilon (( 0.5 \epsilon \lambda^2 u^2 b_{xxx} + 0.5 \lambda b_{xx} u_t
+ \sigma h_{x} ( \epsilon u_{x}^2 - u{x,t}) + \epsilon u (1.5 \lambda b_{xx} u_{x} - s h_x u_{xx} )))
+ \epsilon \sigma^2 h^2 ( \frac{1}{3} \epsilon u_{x}u_{xx}
+ \lambda b_x ( 0.5 \epsilon u_x^2 - 0.5 u_{xt} - 0.5 \epsilon u u_{xx})
- \frac{1}{3} u_{xxt} - \frac{1}{3} \epsilon u u_{xxx})) = 0
$

$\sigma (g + \epsilon^2  \lambda u^2  b_{xx}) h + u^{t}(\epsilon + \epsilon \sigma b_x h_x) + \epsilon^2 u (1 + \sigma b_x h_x) u_x +
\sigma h (\epsilon \lambda b_x^2 (u_t + \epsilon u u_x))
+ b_x (g \lambda + \epsilon(\epsilon \lambda^2 u^2 b_{xx} + 0.5\epsilon u_x^2
+ 0.5 u_{xt} + 0.5 \epsilon u u_{xx} ))
+ \epsilon (( 0.5 \epsilon \lambda^2 u^2 b_{xxx} + 0.5 \lambda b_{xx} u_t
+ \sigma h_{x} ( \epsilon u_{x}^2 - u{x,t}) + \epsilon u (1.5 \lambda b_{xx} u_{x} - s h_x u_{xx} )))
+ \epsilon \sigma^2 h^2 ( \frac{1}{3} \epsilon u_{x}u_{xx}
+ \lambda b_x ( 0.5 \epsilon u_x^2 - 0.5 u_{xt} - 0.5 \epsilon u u_{xx})
- \frac{1}{3} u_{xxt} - \frac{1}{3} \epsilon u u_{xxx}) = 0
$

\begin{multline}
 \left(g + \epsilon^2  \lambda u^2  b_{xx}\right) \sigma h_x + u^{t}(\epsilon + \epsilon \sigma b_x h_x) + \epsilon^2 u (1 + \sigma b_x h_x) u_x 
 \\ +\sigma h (\epsilon \lambda b_x^2 (u_t + \epsilon u u_x))
+ b_x (g \lambda + \epsilon(\epsilon \lambda^2 u^2 b_{xx} + \frac{1}{2}\epsilon u_x^2
 + \frac{1}{2} u_{xt} + \frac{1}{2} \epsilon u u_{xx} ))
 \\
+ \epsilon (( \frac{1}{2} \epsilon \lambda^2 u^2 b_{xxx} + \frac{1}{2} \lambda b_{xx} u_t
+ \sigma h_{x} ( \epsilon u_{x}^2 - u{x,t}) + \epsilon u (1.5 \lambda b_{xx} u_{x} - s h_x u_{xx} ))) 
\\
+ \epsilon \sigma^2 h^2 ( \frac{1}{3} \epsilon u_{x}u_{xx}
+ \lambda b_x ( \frac{1}{2} \epsilon u_x^2 - \frac{1}{2} u_{xt} - \frac{1}{2} \epsilon u u_{xx})
- \frac{1}{3} u_{xxt} - \frac{1}{3} \epsilon u u_{xxx}) = 0
\end{multline}

\begin{multline}
 \left(g + \epsilon^2  \lambda u^2  b_{xx}\right) \sigma h_x + \left(1 + \sigma b_x h_x\right) \epsilon u_{t} +  \left(1 + \sigma b_x h_x \right) \epsilon^2 u u_x
 \\ +\sigma h \left(\epsilon \lambda b_x^2 \left(u_t + \epsilon u u_x \right)\right)
+ b_x \left(g \lambda + \epsilon \left(\epsilon \lambda^2 u^2 b_{xx} + \frac{1}{2}\epsilon u_x^2
 + \frac{1}{2} u_{xt} + \frac{1}{2} \epsilon u u_{xx} \right) \right)
 \\
+ \epsilon \left(\left( \frac{1}{2} \epsilon \lambda^2 u^2 b_{xxx} + \frac{1}{2} \lambda b_{xx} u_t
+ \sigma h_{x} \left( \epsilon u_{x}^2 - u{x,t} \right) + \epsilon u \left(1.5 \lambda b_{xx} u_{x} - s h_x u_{xx} \right)\right)\right) 
\\
+ \epsilon \sigma^2 h^2 \left( \frac{1}{3} \epsilon u_{x}u_{xx}
+ \lambda b_x \left( \frac{1}{2} \epsilon u_x^2 - \frac{1}{2} u_{xt} - \frac{1}{2} \epsilon u u_{xx} \right)
- \frac{1}{3} u_{xxt} - \frac{1}{3} \epsilon u u_{xxx} \right) = 0
\end{multline}

divide $\epsilon$
\begin{multline}
 \left(\frac{g}{\epsilon} + \epsilon  \lambda u^2  b_{xx}\right) \sigma h_x + \left(1 + \sigma b_x h_x\right) u_{t} +  \left(1 + \sigma b_x h_x \right) \epsilon u u_x
 \\ +\sigma h\lambda b_x^2 \left(u_t + \epsilon u u_x \right)
+ b_x \left( \frac{g \lambda}{\epsilon} +  \epsilon \lambda^2 u^2 b_{xx} + \frac{1}{2}\epsilon u_x^2
 + \frac{1}{2} u_{xt} + \frac{1}{2} \epsilon u u_{xx}  \right)
 \\
+  \frac{1}{2} \epsilon \lambda^2 u^2 b_{xxx} + \frac{1}{2} \lambda b_{xx} u_t
+ \sigma h_{x} \left( \epsilon u_{x}^2 - u_{xt} \right) + \epsilon u \left(1.5 \lambda b_{xx} u_{x} - s h_x u_{xx} \right)
\\
+ \sigma^2 h^2 \left( \frac{1}{3} \epsilon u_{x}u_{xx}
+ \lambda b_x \left( \frac{1}{2} \epsilon u_x^2 - \frac{1}{2} u_{xt} - \frac{1}{2} \epsilon u u_{xx} \right)
- \frac{1}{3} u_{xxt} - \frac{1}{3} \epsilon u u_{xxx} \right) = 0
\end{multline}




\end{document}
